\section*{Problem 3}

\begin{enumerate}
\item
We first define the extended state $x_e(k) = [x^T(k) \ x_f^T(k)]^T$ so that the system and cost function dynamics can be written
\begin{align}
    x_e(k+1) & = A_e x_e(k) + B_e u(k) 
        \label{eq:m1p3_syse1} \\
    y_f(k) & = C_e x_e(k)
        \label{eq:m1p3_syse2}
\end{align}
where
\begin{align*}
    A_e & = \begin{bmatrix}
            A & 0 \\
            B_f C & A_f
        \end{bmatrix}
        & B_e & = \begin{bmatrix}
            B \\
            0
        \end{bmatrix}
        & C_e & = \begin{bmatrix}
            D_f C & C_f 
        \end{bmatrix}
        & x_e(0) & = \begin{bmatrix}
            x(0) \\
            0
        \end{bmatrix}
\end{align*}
With this, the cost function can now be written as
\begin{align}
    J = x_e^T(N) C_e^T C_e x_e(N) + \sum_{k=0}^{N-1} \left[ x_e^T(k) C_e^T C_e x_e(k) + u^T(k) R u(k) \right]
        \label{eq:m1p3_cost}
\end{align}
We now note that minimizing \eqref{eq:m1p3_cost} subject to \eqref{eq:m1p3_syse1}--\eqref{eq:m1p3_syse2} is a standard LQR problem. We can therefore immediately write down the solution:
\begin{align*}
    u_1^o(k) & = -K(k+1) x_e(k) \\
    K(k) & = [B_e^T P(k) B_e + R]^{-1} B_e^T P(k) A_e \\
    P(k-1) & = A_e^T P(k) A_e + C_e^T C_e - A_e^T P(k) B_e [ B_e^T P(k) B_e + R]^{-1} B_e^T P(k) A_e \\
    P(N) & = C_e^T C_e
\end{align*}
The corresponding optimal cost is
\begin{align*}
    J^o = x_e^T(0) P(0) x_e(0)
\end{align*}



\item
We first partition $K(k) = [K_x(k) \ K_f(k)]$ so that the optimal control law from the previous part can be written as
\begin{align*}
    u_1^o(k) = -K_x(k+1) x(k) - K_f(k+1) x_f(k)
\end{align*}
Now we note that the value of $x_f(k)$ can be constructed from $x(0),\ldots,x(k-1)$ using the recursive relationship
\begin{align*}
    x_f(k+1) & = A_f x_f(k) + B_f C x(k),
        & x_f(0) & = 0
\end{align*}
With this, we see that $u_1^o(k)$ can be regarded as a function of $x(0),\ldots,x(k)$. In particular,
\begin{align*}
    x_f(k+1) & = A_f x_f(k) + B_f C x(k),
        & x_f(0) & = 0 \\
    u_2^o(k) & = -K_f(k+1) x_f(k) - K_x(k+1) x(k)
\end{align*}
Note that the optimal control law is expressed as the output of a state space model with input $x(k)$. Since $u_1^o(k) = u_2^o(k)$, the optimal cost is the same as in the previous part, i.e.\ $J^o = x_e^T(0) P(0) x_e(0)$.

\end{enumerate}


